io/case-studies/webserver/MonitorParam.fst
@@ -1,0 +1,130 @@
+module MonitorParam
+
+open FStar.Tactics
+open FStar.List.Tot
+open MIO.Sig
+
+let rec is_opened_by_untrusted (h:trace) (fd:file_descr) : bool =
+  match h with
+  | [] -> false
+  | EOpenfile Ctx _ res :: tl ->
+    if Inl? res && fd = Inl?.v res then true
+    else is_opened_by_untrusted tl fd
+  | EClose _ fd' res :: tl ->
+    if Inl? res && fd = fd' then false
+    else is_opened_by_untrusted tl fd
+  | e :: tl -> is_opened_by_untrusted tl fd
+
+val wrote_to : file_descr -> trace -> bool
+let rec wrote_to client h =
+  match h with
+  | [] -> false
+  | EAccept _ arg res :: tl -> begin
+    match res with
+    | Inl fd -> if fd = client then false else wrote_to client tl
+    | _ -> wrote_to client tl
+  end
+  | EWrite Prog arg _ :: tl ->
+    let (fd, _) = arg in
+    if fd = client then true
+    else wrote_to client tl
+  | _ :: tl -> wrote_to client tl
+
+let rec did_not_respond (h:trace) : bool =
+  match h with
+  | [] -> false
+  | ERead Prog _ _ :: tl -> true
+  | EWrite Prog _ _ :: tl -> false
+  | e :: tl -> did_not_respond tl
+
+type status =
+| DidNotRespond
+| Responded
+
+let models_status (c:status) (h:trace) : bool =
+  match c with
+  | DidNotRespond -> did_not_respond h
+  | Responded -> not (did_not_respond h)
+
+noeq type cst = {
+  opened : list file_descr ;
+  st : status ;
+  written : list file_descr
+}
+
+
+let models (c : cst) (h : trace) : Type0 =
+  c.st `models_status` h /\
+  (forall fd. fd `mem` c.opened <==> is_opened_by_untrusted h fd) /\
+  (forall fd. fd `mem` c.written <==> wrote_to fd h)
+
+let mymst : mstate = {
+  typ = cst;
+  abstracts = models;
+}
+
+let mkcst x y z = {
+  opened = x ;
+  st = y ;
+  written = z
+}
+
+let my_init_cst : mymst.typ =
+  mkcst [] Responded []
+
+let updst (c : cst) s : cst = {
+  opened = c.opened ;
+  st = s ;
+  written = c.written
+}
+
+let open_cst (fd : file_descr) (c : cst) : cst = {
+  opened = fd :: c.opened ;
+  st = c.st ;
+  written = c.written
+}
+
+let write_cst (fd : file_descr) (c : cst) : cst = {
+  opened = c.opened ;
+  st = Responded ;
+  written = fd :: c.written
+}
+
+let is_neq (#a:eqtype) (x y : a) : bool = x <> y
+
+let close_cst (fd : file_descr) (c : cst) : cst = {
+  opened = filter (is_neq fd) c.opened ;
+  st = c.st ;
+  written = c.written
+}
+
+let accept_cst (fd : file_descr) (c : cst) : cst = {
+  opened = c.opened ;
+  st = c.st ;
+  written = filter (is_neq fd) c.written
+}
+
+
+let my_update_cst (s0:cst) (e:event) : (s1:cst{forall h. s0 `models` h ==> s1 `models` (e::h)}) =
+  let (| caller, cmd, arg, res |) = destruct_event e in
+  match cmd, res with
+  | Accept, Inl fd ->
+    mem_filter_equiv (is_neq fd) s0.written ;
+    accept_cst fd s0
+  | Read, _ ->
+    let (fd, _) : file_descr * UInt8.t = arg in
+    if caller = Prog then updst s0 DidNotRespond else s0
+  | Openfile, Inl fd -> if caller = Ctx then open_cst fd s0 else s0
+  | Close, Inl rr ->
+    mem_filter_equiv (is_neq arg) s0.opened ;
+    close_cst arg s0
+  | Write, _ ->
+    let arg : file_descr * Bytes.bytes = arg in
+    let (fd, bb) = arg in
+    if caller = Prog then write_cst fd s0 else s0
+  | _ -> s0
+
+let mymst_impl : mst_impl mymst = {
+  init = my_init_cst;
+  update = (fun s e h -> my_update_cst s e);
+}
